WIP: substitution lemmas and logical relations

src/Compatibility.v
@@ -2,23 +2,23 @@ Require Import LogRel.
 Import ListNotations.
 
 Lemma Vrel_Var_compat :
-  forall Γ x,
-  In (inl x) Γ ->
-  Vrel_open Γ (EVar x) (EVar x).
+  forall Γ n x,
+  n < Γ ->
+  Vrel_open Γ (EVar n x) (EVar n x).
 Proof.
-  unfold Vrel_open, Grel.
-  cbn. intuition.
+  unfold Vrel_open, Grel. intros. destruct H0, H1. simpl subst. specialize (H2 n H).
+  repeat break_match_hyp; auto; contradiction.
 Qed.
 
 Hint Resolve Vrel_Var_compat.
 
 Lemma Vrel_FunId_compat :
-  forall Γ x,
-  In (inr x) Γ ->
-  Vrel_open Γ (EFunId x) (EFunId x).
+  forall Γ n x,
+  n < Γ ->
+  Vrel_open Γ (EFunId n x) (EFunId n x).
 Proof.
-  unfold Vrel_open, Grel.
-  cbn. intuition.
+  unfold Vrel_open, Grel. intros. destruct H0, H1. simpl subst. specialize (H2 n H).
+  repeat break_match_hyp; auto; contradiction.
 Qed.
 
 Hint Resolve Vrel_FunId_compat.
@@ -41,271 +41,26 @@ Qed.
 
 Hint Resolve Vrel_Lit_compat_open.
 
-Definition composition {A B C : Type} (f : B -> C) (g : A -> B) : A -> C := fun x => f (g x).
-
-Lemma compose_subst :
-  forall ξ₁ ξ₂ e, subst ξ₁ (subst ξ₂ e) = composition (subst ξ₁) (subst ξ₂) e.
-Proof.
-  intros. unfold composition. reflexivity.
-Qed.
-
-(* Lemma subst_composition :
-  forall e ξ l vals Γ, length l = length vals -> subscoped Γ [] ξ ->
-  EXP Γ ++ l ⊢ e ->
-  composition (subst (idsubst[[ ::= combine l vals]])) (subst (ξ -- l)) e = subst (ξ[[::= combine l vals]]) e.
-Proof.
-  induction e; intros; unfold composition; simpl; auto.
-  * unfold "--". simpl. destruct (in_list (inl v) l) eqn:P.
-    - simpl. apply subst_list_in; auto. apply in_list_sound in P. auto. 
-    - inversion H1. inversion H2. subst. apply not_in_list_sound in P.
-      apply in_app_iff in H5. destruct H5. 2: contradiction.
-      rewrite subst_list_not_in; auto.
-      specialize (H0 _ H3). eapply vclosed_ignores_sub in H0. rewrite H0. reflexivity.
-  * unfold "--". simpl. destruct (in_list (inr f) l) eqn:P.
-    - simpl. apply subst_list_in; auto. apply in_list_sound in P. auto. 
-    - inversion H1. inversion H2. subst. apply not_in_list_sound in P.
-      apply in_app_iff in H5. destruct H5. 2: contradiction.
-      rewrite subst_list_not_in; auto.
-      specialize (H0 _ H3). eapply vclosed_ignores_sub in H0. rewrite H0. reflexivity.
-  * assert ((subst ((idsubst [[ ::= combine l vals]]) -- map inl vl) (subst ((ξ -- l) -- map inl vl) e)) = (subst ((ξ [[ ::= combine l vals]]) -- map inl vl) e)).
-    { unfold composition in IHe.
-Abort. *)
-
-Definition varname (e : Exp) : option VarFunId :=
-match e with
-| EVar v   => Some (inl v)
-| EFunId f => Some (inr f)
-| _        => None
-end.
-
-Definition substcomp (ξ η : Substitution) : Substitution :=
-  composition (subst ξ) η.
-(* fun x =>
-  match (varname (η x)) with
-  | Some vname => ξ vname
-    (* if var_funid_eqb vname x
-    then ξ x
-    else η x *)
-  | _ => η x
-end. *)
-(* 
-Lemma idsubst_varname : forall x, varname (idsubst x) = Some x.
-Proof.
-  intros. destruct x; cbn; auto.
-Qed.
-*)
-
-Lemma subst_restrict_app :
-  forall ξ l1 l2, ((ξ -- l1) -- l2) = (ξ -- (l1 ++ l2)).
-Proof.
-  intros. extensionality x. unfold "--". break_match_goal.
-  * apply in_list_sound in Heqb. eapply in_app_right in Heqb.
-    apply in_list_sound in Heqb. rewrite Heqb. auto.
-  * break_match_goal.
-    - apply in_list_sound in Heqb0. eapply in_app_left in Heqb0.
-      apply in_list_sound in Heqb0. rewrite Heqb0. auto.
-    - apply not_in_list_sound in Heqb. apply not_in_list_sound in Heqb0.
-      eapply app_not_in in Heqb; eauto. apply not_in_list_sound in Heqb. rewrite Heqb. auto.
-Qed.
-
-(* Lemma subst_composition :
-  forall e ξ η l,
-  (subst (η[[::= l]])) (subst (ξ -- fst (split l)) e) = 
-  subst (substcomp (η[[::= l]]) (ξ -- fst (split l))) e.
-Proof.
-  induction e; intros; auto; simpl.
-  * Search "--". rewrite subst_restrict_app.
-Abort. *)
-
-(** In general, the following lemma could not be weakened more:
-    (ξ₁ -- l) cannot be replaced by ξ₁ on the right-hand side.
-*)
-Lemma substcomp_restrict : forall ξ₁ ξ₂ l,
-  (substcomp (ξ₁ -- l) (ξ₂ -- l)) = (substcomp (ξ₁ -- l) ξ₂ -- l).
-Proof.
-  intros. unfold "--". extensionality x.
-  break_match_goal; cbn.
-  * rewrite Heqb. destruct x; simpl; break_match_goal; auto.
-    - apply in_list_sound in Heqb. apply not_in_list_sound in Heqb0. contradiction. (* Coq bug *)
-    - apply in_list_sound in Heqb. apply not_in_list_sound in Heqb0. contradiction.
-  * rewrite Heqb. unfold substcomp, composition. reflexivity.
-Qed.
-
-(*
-    What if ξ₂ produced closed values? Or just ξ₂'s result is NOT containing any
-    variables of l?
-*)
-Lemma substcomp_restrict_x : forall ξ₁ ξ₂ l x, VALCLOSED (ξ₂ x) ->
-  (substcomp (ξ₁ -- l) (ξ₂ -- l)) x = (substcomp ξ₁ ξ₂ -- l) x.
-Proof.
-  intros. rewrite substcomp_restrict. unfold substcomp, "--", composition.
-  break_match_goal; auto.
-  eapply vclosed_ignores_sub in H as H'. rewrite H'.
-  eapply vclosed_ignores_sub in H. rewrite H. auto.
-Qed.
-
-(* Lemma subscoped_app_restrict : forall Γ ξ Γ' l,
-  subscoped Γ Γ' ξ -> subscoped (Γ ++ l) Γ' (ξ -- l).
-Proof.
-  intros. unfold subscoped in *. intros. unfold "--". break_match_goal.
-Abort. *)
-(* 
-Fixpoint bound_variables (e : Exp) : list VarFunId :=
-match e with
- | ELit l => []
- | EVar v => []
- | EFunId f => []
- | EFun vl e => map inl vl ++ bound_variables e
- | ERecFun f vl e => inr f :: map inl vl ++ bound_variables e
- | EApp exp l => bound_variables exp ++ fold_left (fun acc e => bound_variables e ++ acc) l []
- | ELet v e1 e2 => inl v :: bound_variables e1 ++ bound_variables e2
- | ELetRec f vl b e => inr f :: map inl vl ++ bound_variables b ++ bound_variables e
- | EPlus e1 e2 => bound_variables e1 ++ bound_variables e2
- | EIf e1 e2 e3 => bound_variables e1 ++ bound_variables e2 ++ bound_variables e3
-end.
-
-Fixpoint free_variables (e : Exp) : list VarFunId :=
-match e with
- | ELit l => []
- | EVar v => [inl v]
- | EFunId f => [inr f]
- | EFun vl e => filter (fun name => negb (in_list name (map inl vl))) (free_variables e)
- | ERecFun f vl e => filter (fun name => negb (in_list name (inr f :: map inl vl))) (free_variables e)
- | EApp exp l => free_variables exp ++ fold_left (fun acc e => free_variables e ++ acc) l []
- | ELet v e1 e2 => free_variables e1 ++ filter (fun name => negb (var_funid_eqb name (inl v))) (free_variables e2)
- | ELetRec f vl b e => filter (fun name => negb (in_list name (inr f :: map inl vl))) (free_variables b) ++ filter (fun name => negb (var_funid_eqb name (inr f))) (free_variables e)
- | EPlus e1 e2 => free_variables e1 ++ free_variables e2
- | EIf e1 e2 e3 => free_variables e1 ++ free_variables e2 ++ free_variables e3
-end.
-
-Compute free_variables (sum 114).
-
-Local Definition l1 := ELet "X"%string (EVar "X"%string) (EVar "X"%string).
-Compute bound_variables l1.
-
-Definition capture_avoiding_subst (l : list VarFunId) (ξ : Substitution) :=
-  forall x, filter (fun name => in_list name l) (free_variables (ξ x)) = []. *)
-
-Corollary substcomp_restrict_subscoped : forall e ξ₁ ξ₂ l Γ, subscoped Γ [] ξ₂ ->
-  EXP Γ ⊢ e ->
-  subst (substcomp (ξ₁ -- l) (ξ₂ -- l)) e = subst (substcomp ξ₁ ξ₂ -- l) e.
-Proof.
-  induction e; intros; simpl; auto.
-  * apply substcomp_restrict_x. apply H. inversion H0. inversion H1. auto.
-  * apply substcomp_restrict_x. apply H. inversion H0. inversion H1. auto.
-  * inversion H0. inversion H1. subst.
-    rewrite subst_restrict_comm. erewrite <- IHe.
-    rewrite subst_restrict_comm. replace ((ξ₂ -- l) -- map inl vl) with ((ξ₂ -- map inl vl) -- l). 2: apply subst_restrict_comm. repeat rewrite subst_restrict_app. erewrite IHe.
-    auto.
-  
-(* (*     rewrite subst_restrict_comm, substcomp_restrict, subst_restrict_comm. erewrite IHe. 3: eauto.
-    subst_restrict_comm. auto. *) *)
-Abort.
-
-(**
-  with capture-avoiding substitution, this should be trivial
-
-  However, if we substitute bound variables to closed values, it should not be a problem.
-*)
-Lemma subst_composition2 :
-  forall e ξ₁ ξ₂ Γ, EXP Γ ⊢ e -> subscoped Γ [] ξ₂ ->
-  (subst ξ₁) (subst ξ₂ e) = subst (substcomp ξ₁ ξ₂) e.
-Proof.
-  induction e; intros; simpl; auto.
-  * erewrite IHe.
-Admitted.
-
-(* Lemma subst_composition_scoped :
-  forall ξ η Γ Γ', subscoped Γ Γ' ξ -> subscoped Γ Γ' η -> subscoped Γ Γ' (substcomp ξ η).
-Proof.
-(*   intros. intro. intros. unfold substcomp. break_match_goal;
-  [ apply H | apply H0 ]; auto. *)
-  
-Abort. *)
-
-Lemma subst_list_in_val : forall l x vals ξ, length l = length vals ->
-  In x l -> exists v, In v vals /\ (ξ[[ ::= combine l vals]]) x = v.
-Proof.
-  induction l; intros.
-  * inversion H0.
-  * apply element_exist in H as H0'. destruct H0', H1. subst. inversion H.
-    unfold extend_subst. destruct (in_dec var_funid_eq_dec x l).
-    - epose (IHl x x1 _ H2 i). destruct e, H1. exists x2. split. firstorder.
-      simpl. eexact H3.
-    - inversion H0. 2: contradiction. subst.
-      exists x0. split. firstorder. simpl.
-      repeat rewrite subst_list_not_in; auto.
-      unfold extend_subst. rewrite var_funid_eqb_refl. auto.
-Qed.
-
-(* Lemma subscoped_ext_app :
-  forall ξ Γ Γ' l vals, subscoped Γ Γ' ξ -> length l = length vals ->
-  Forall (fun v => VAL Γ' ⊢ v ) vals ->
-  subscoped (Γ ++ l) Γ' (substcomp (idsubst[[::= combine l vals]]) (ξ -- l)).
-Proof.
-  intros. intro. intros. unfold "--", substcomp. (* break_match_goal.
-  * break_match_hyp.
-    - apply in_list_sound in Heqb. Check subst_list_in.
-      epose (subst_list_in_val _ _ _ _ H0 Heqb). destruct e. destruct H3.
-      rewrite H4. rewrite indexed_to_forall in H1. (* Just technical, but doable *) *)
-Admitted. *)
-
-Lemma biforall_vrel_helper : forall m vals1 vals2, length vals1 = length vals2 ->
-  list_biforall (Vrel m) vals1 vals2 ->
-  Forall (fun v : Exp => VALCLOSED v) vals1 /\
-  Forall (fun v : Exp => VALCLOSED v) vals2.
-Proof.
-  induction vals1; intros.
-  * apply eq_sym, length_zero_iff_nil in H. subst. firstorder.
-  * apply element_exist in H as H'. destruct H', H1. subst. inversion H.
-    inversion H0. subst. apply Vrel_closed in H5. destruct H5.
-    split; constructor; auto.
-    - apply (IHvals1 x0); auto.
-    - apply (IHvals1 x0); auto.
-Qed.
-
-(* Lemma alma :
-  forall e ξ x v, 
-                  subst (idsubst[[x ::= v]]) (subst (ξ -- [x]) e) =
-                  subst (ξ[[x ::= v]]) e.
-Proof.
-  induction e; intros; subst; try reflexivity.
-  * unfold "--", extend_subst. cbn. break_match_goal.
-    - break_match_goal.
-      + apply var_funid_eqb_eq in Heqb0. subst. cbn. rewrite eqb_refl. auto.
-      + apply var_funid_eqb_neq in Heqb0. break_match_hyp.
-        ** destruct x.
-           -- apply eqb_eq in Heqb1. subst. contradiction.
-           -- congruence.
-        ** congruence.
-    - break_match_goal.
-      + apply var_funid_eqb_eq in Heqb0. subst. rewrite eqb_refl in Heqb. congruence.
-      + break_match_hyp.
-        ** congruence.
-        ** destruct x.
-           -- apply 
-Qed. *)
-
 Lemma Vrel_Fun_compat :
-  forall Γ vl b1 b2,
-  Erel_open (Γ ++ map inl vl) b1 b2 ->
-  Vrel_open Γ (EFun vl b1) (EFun vl b2).
+  forall Γ vl1 vl2 b1 b2, length vl1 = length vl2 ->
+  Erel_open (length vl1 + Γ) b1 b2 ->
+  Vrel_open Γ (EFun vl1 b1) (EFun vl2 b2).
 Proof.
   intros. unfold Vrel_open. intros.
-  inversion H0 as [? [? ?] ].
+  inversion H1 as [? [? ?] ].
   simpl. rewrite Vrel_Fix_eq. unfold Vrel_rec at 1. intuition idtac.
-  - constructor. eapply subst_preserves_scope_rev; eauto.
-  - constructor. eapply subst_preserves_scope_rev; eauto.
-  - break_match_goal; try congruence. intros. unfold Erel_open, Erel in H.
-    Search subst.
-(*     rewrite subst_composition; eauto.
-    unfold Erel in H.
-    eapply H. unfold Grel. split. 2: split.
-    1-2: apply subscoped_ext_app; auto.
-    1, 3: rewrite map_length; auto.
-    1-2: apply biforall_vrel_helper in H6.
-    1-4: try lia; destruct H6; auto.
-    intros. unfold substcomp. (* Technical, but doable *)*)
+  - constructor. Search Erel ExpScoped. rewrite Nat.add_0_r. eapply Erel_open_scope in H0.
+    destruct H0. eapply subst_preserves_scope_exp in H0. exact H0.
+    Search subscoped. replace (length vl1) with (length vl1 + 0) at 2 by lia. eapply upn_scope. auto.
+  - constructor. Search Erel ExpScoped. rewrite Nat.add_0_r. eapply Erel_open_scope in H0.
+    destruct H0. rewrite H in H5. eapply subst_preserves_scope_exp in H5. exact H5.
+    Search subscoped. replace (length vl2) with (length vl2 + 0) at 2 by lia. eapply upn_scope. auto.
+  - break_match_goal.
+    + intros. unfold Erel_open, Erel in H0.
+      rewrite substcomp_subst, substcomp_subst. apply H0.
+      split. 2: split.
+      * Search upn subscoped.
+    + apply Nat.eqb_neq in Heqb. contradiction.
 Admitted.
 
 Lemma Vrel_RecFun_compat :
@@ -474,3 +229,57 @@ Qed.
 Hint Resolve Vrel_open_Erel_open.
 *)
 
+Theorem Vrel_Fundamental_closed :
+  forall (v : Exp),
+    VALCLOSED v ->
+    forall n, Vrel n v v.
+Proof.
+Admitted.
+
+Theorem exp_rel_trans :
+  forall n vrel e1 e2 e3,
+    exp_rel n vrel e1 e2 -> exp_rel n vrel e2 e3 -> exp_rel n vrel e1 e3.
+Proof.
+  intros. unfold exp_rel in *. destruct H, H0, H1, H2. intuition.
+  specialize (H3 _ Hmn _ H5). destruct H3, H3, H3.
+Abort.
+
+Theorem Vrel_closed_trans :
+  forall n (v1 v2 v3 : Exp),
+    Vrel n v1 v2 -> Vrel n v2 v3 -> Vrel n v1 v3.
+Proof.
+  induction n.
+  {
+  intros.
+  rewrite Vrel_Fix_eq in H. rewrite Vrel_Fix_eq in H0. rewrite Vrel_Fix_eq.
+  destruct v1.
+  2-3, 6-10: inversion H; inversion H2; contradiction.
+  all: destruct v2.
+  all: try inversion H; try inversion H2; try contradiction.
+  all: destruct v3.
+  all: try inversion H0; try inversion H6; try contradiction.
+  all: subst.
+  * unfold Vrel_rec. split. 2: split. all: constructor.
+  * clear H2 H6. break_match_hyp. break_match_hyp. 2-3: contradiction.
+    subst. unfold Vrel_rec. intuition. break_match_goal. 2: contradiction. intros. inversion Hmn.
+  * clear H2 H6. break_match_hyp. break_match_hyp. 2-3: contradiction.
+    subst. unfold Vrel_rec. intuition. break_match_goal. 2: contradiction. intros. inversion Hmn.
+  }
+  {
+  intros.
+  rewrite Vrel_Fix_eq in H. rewrite Vrel_Fix_eq in H0. rewrite Vrel_Fix_eq.
+  destruct v1.
+  2-3, 6-10: inversion H; inversion H2; contradiction.
+  all: destruct v2.
+  all: try inversion H; try inversion H2; try contradiction.
+  all: destruct v3.
+  all: try inversion H0; try inversion H6; try contradiction.
+  all: subst.
+  * unfold Vrel_rec. split. 2: split. all: constructor.
+  * clear H2 H6. break_match_hyp. break_match_hyp. 2-3: contradiction.
+    subst. unfold Vrel_rec. intuition. break_match_goal. 2: contradiction. intros.
+    specialize (H8 m Hmn vals1 vals2 H2 H6 H9).
+    specialize (H4 m Hmn vals1 vals2 H2 H6 H9). admit.
+  * admit.
+  }
+Admitted.
